\begin{align*}
    \div{\vec{D}} =& \rho_{f} \\
    \div{\vec{B}} =& 0 \\
    \curl{\vec{E}} =& \pd{\vec{B}}{t} \\
    \curl{\vec{H}} =& \vec{J}_{f} + \pd{\vec{D}}{t}
\end{align*}

\begin{align*}
    \vec{D} =& \epsilon_{0}\vec{E} + \vec{P} \\
    \vec{B} =& \mu_{0}(\vec{H} + \vec{M})
\end{align*}

\begin{align*}
    \closedintegral{\vec{D}}{\vec{a}} =& Q_{f,enc} \\
    \closedintegral{\vec{H}}{\vec{l}} =& I_{f,enc}(t) + \d{\Phi_{\vec{D}}}{t} \\
    \closedintegral{\vec{B}}{\vec{a}} =& 0\\
    \closedintegral{\vec{E}}{\vec{l}} =& - \d{\Phi_{\vec{B}}}{t}
\end{align*}

\begin{align*}
    D_{1}^{\perp} - D_{2}^{\perp} &= \sigma_{f} \\
    B_{1}^{\perp} - B_{2}^{\perp} &= 0 \\
    \vec{E}_{1}^{\parallel} - \vec{E}_{2}^{\parallel} &= 0 \\
    \vec{H}_{1}^{\parallel} - \vec{H}_{2}^{\parallel} &= \vec{K}_f \times \hat{\vec{n}}
\end{align*}

\begin{align*}
    \vec{S} =& \frac{1}{\mu} \vec{E} \times \vec{B} \\
    u =& \frac{1}{2} \left( \epsilon_0 E^{2} + \frac{1}{\mu_0} B^{2} \right) \\
    I =& \langle S \rangle = \frac{1}{2} v\epsilon E_{0}^{2} \\
    P =& \int \vec{S} \cdot \mathrm{d}\vec{a}
\end{align*}

\subsection{Special Relativity}
\begin{equation*}
    \Lambda =
    \begin{pmatrix}
        \gamma & -\beta\gamma & 0 & 0 \\
        -\beta\gamma & \gamma & 0 & 0 \\
        0 & 0 & 1 & 0 \\
        0 & 0 & 0 & 1
    \end{pmatrix}
\end{equation*}

\begin{equation*}
    u^{\prime} = \frac{u - v}{1 - \frac{uv}{c^{2}}}
\end{equation*}

\begin{equation*}
    \Lambda^{\mu}_{\alpha} g_{\mu\nu} \Lambda^{\nu}_{\beta} = g_{\alpha\beta}
\end{equation*}

\begin{equation*}
    I = s^{2} = x_{\mu}x^{\mu} = c^{2}t^{2} - d^{2}
\end{equation*}

\begin{align*}
    \mathrm{d}\tau &= \frac{\mathrm{d}t}{\gamma} \comment{proper time} \\
    \eta^{\mu} &= \d{x^{\mu}}{\tau} =
    \begin{pmatrix}
        \gamma c \\
        \gamma \vec{u}
    \end{pmatrix}\comment{proper velocity} \\
    \eta^{\mu} &= m\eta^{\mu} =
    \begin{pmatrix}
        E/c \\
        \vec{p}
    \end{pmatrix}\comment{proper velocity}
\end{align*}

\begin{align*}
    \eta_{\mu}\eta^{\mu} &= c^{2} \\
    p_{\mu}p^{\mu} &= E^{2}/c^{2} - \vec{p}^{2} = m^{2}c^{2}\\
\end{align*}

\begin{equation*}
    F^{\mu\nu} =
    \begin{pmatrix}
        0 & -E_{x}/c & -E_{y}/c & -E_{z}/c \\
        E_{x}/c & 0 & -B_{z} & B_{y} \\
        E_{y}/c & B_{z} & 0 & -B_{x} \\
        E_{z}/c & -B_{y} & B_{x} & 0
    \end{pmatrix}
\end{equation*}

\begin{equation*}
    K^{\mu} = q F^{\mu\nu} g_{\nu\alpha} \eta^{\alpha}
\end{equation*}

\begin{equation*}
    J^{\mu} =
    \begin{pmatrix}
        c\rho \\
        \vec{J}
    \end{pmatrix}
\end{equation*}

\begin{equation*}
    \partial_{\mu}J^{\mu} = 0
\end{equation*}

\begin{equation*}
    \vec{A}(\vec{x}) = \frac{1}{4\pi} \int \frac{\nabla^{\prime} \times \vec{J}({\vec{x}^{\prime})}}{|\vec{x} - \vec{x}^{\prime}|} \mathrm{d}\vec{x}
\end{equation*}

\begin{align*}
    \vec{B} &= \curl{A}\\
    \vec{E} &= -\grad{V} - \pd{\vec{A}}{t}
\end{align*}

\begin{equation*}
    A^{\mu}_{\text{ret}}(\vec{x}) = \frac{\mu_0}{4\pi} \int \mathrm{d}^{3}x^{\prime}
    \frac{J^{\prime}(x^{0} - |\vec{x} - \vec{x}^{\prime}, \vec{x}^{\prime})}{|\vec{x} - \vec{x}^{\prime}|}
\end{equation*}

\subsection{Radiation}

\begin{align*}
    \vec{E} &= \frac{q}{4\pi \epsilon}
    \Bigl(\frac{\hat{\vec{r}} - \vec{\beta}}{\gamma^{2} (1 - \vec{\beta}\cdot\hat{\vec{r}})^{3} |\vec{r}|^{2}} \\
        &+\frac{\hat{\vec{r}} \times ((\hat{\vec{r}} - \vec{\beta}) \times \dot{\vec{\beta}})}{(1- \vec{\beta}\cdot\hat{\vec{r}})^{3}c|\vec{r}|}\Bigr) \comment{for point charge}
\end{align*}

\begin{equation*}
    \vec{E} = \frac{q}{4\pi\epsilon_{0}} \frac{\hat{\vec{r}} - \vec{\beta}}{\gamma^{2} (1-\vec{\beta}\cdot\hat{\vec{r}})^{3}|\vec{r}|^{2}} \comment{constant velocity}
\end{equation*}

\begin{equation*}
    \d{P}{\Omega} = \frac{\mu_{0} q^{2}}{16\pi c}
    \frac{(\hat{\vec{r}} \times ((\hat{\vec{r}} - \vec{\beta}) \times \vec{a}))^{2}}
    {(1 - \vec{\beta} \cdot \hat{\vec{r}})^{5}}
\end{equation*}

\begin{align*}
    \d{P}{\Omega} = \frac{\mu_{0} q^{2} a^{2}}{16 \pi^{2}c} \sin^{2}\theta \comment{non-rel. limit} \\
    P = \frac{\mu_{0} q^{2} a^{2}}{6 \pi c}
\end{align*}

\begin{equation*}
    P = \frac{\mu_{0} q^{2} \gamma^{2}}{6 \pi c} (a^{2} - |\vec{\beta} \times \vec{a}|^{2}) \comment{rel. generalisation}
\end{equation*}

todo Maybe do dipole stuff?
\subsection{Radiation of dipole}
\begin{equation}
    \vec{p}(t) = e^{-i \omega t}\int \rho{\vec{x}^{\prime}} \vec{x}^{\prime} \mathrm{d}^{3}x^{\prime} \comment{dipole moment}
\end{equation}

